Fresh snapshot

Source/DafnyStandardLibraries/src/Std/Actions/Actions.dfy
@@ -1,22 +1,21 @@
 
-module {:options "--function-syntax:4"} Std.Actions {
+module Std.Actions {
 
   import opened Wrappers
   import opened Frames
-  import opened Collections.Seq
-  import opened Math
   import opened GenericActions
   import opened Termination
   import opened DynamicArray
+  import Collections.Seq
 
   // TODO: Documentation, especially overall design
   trait {:termination false} Action<T, R> extends GenericAction<T, R>, Validatable {
 
     ghost var history: seq<(T, R)>
 
-    ghost predicate Valid() 
-      reads this, Repr 
-      ensures Valid() ==> this in Repr 
+    ghost predicate Valid()
+      reads this, Repr
+      ensures Valid() ==> this in Repr
       ensures Valid() ==> CanProduce(history)
       decreases height, 0
 
@@ -30,6 +29,9 @@ module {:options "--function-syntax:4"} Std.Actions {
     //
     // The downside is that these are then forced to use quantifiers
     // to talk about all possible states of an action.
+    // The solution is the trait proof pattern,
+    // where a trait is passed around with an abstract lemma
+    // that can be invoked on the otherwise quantified state as needed.
 
     // TODO: Necessary but not sufficient that:
     // CanConsume(history, nextIn) ==> exists nextOut :: CanProduce(history + [(nextIn, nextOut)])
@@ -71,6 +73,21 @@ module {:options "--function-syntax:4"} Std.Actions {
       && fresh(Repr - old(Repr))
     }
 
+    // Possibly optimized extensions
+
+    // Equivalent to DefaultRepeatUntil below, but may be implemented more efficiently.
+    method RepeatUntil(t: T, stop: R -> bool, ghost eventuallyStopsProof: ProducesTerminatedProof<T, R>)
+      requires Valid()
+      requires eventuallyStopsProof.Action() == this
+      requires eventuallyStopsProof.FixedInput() == t
+      requires eventuallyStopsProof.StopFn() == stop
+      requires forall i <- Consumed() :: i == t
+      reads Reads(t)
+      modifies Repr
+      decreases Repr
+      ensures Valid()
+      //ensures history == old(history) + (n copies of t)/(n - 1 not stop values + stop)
+
     // Helpers
 
     ghost method Update(t: T, r: R)
@@ -94,6 +111,55 @@ module {:options "--function-syntax:4"} Std.Actions {
     }
   }
 
+  method DefaultRepeatUntil<T, R>(a: Action<T, R>, t: T, stop: R -> bool, ghost eventuallyStopsProof: ProducesTerminatedProof<T, R>) 
+    requires a.Valid()
+    requires eventuallyStopsProof.Action() == a
+    requires eventuallyStopsProof.FixedInput() == t
+    requires eventuallyStopsProof.StopFn() == stop
+    requires forall i <- a.Consumed() :: i == t
+    reads a.Repr
+    modifies a.Repr
+    ensures a.Valid()
+  {
+    // TODO: loops need to support reads clauses as well!
+
+    while (true) 
+      modifies a.Repr
+      invariant a.Valid()
+      invariant fresh(a.Repr - old(a.Repr))
+      invariant forall i <- a.Consumed() :: i == t
+      decreases eventuallyStopsProof.Remaining()
+    {
+      label beforeInvoke:
+      assert a.Valid();
+      assert a.CanProduce(a.history);
+      eventuallyStopsProof.CanConsumeAll(a.history, t);
+      assert a.CanConsume(a.history, t);
+      var next := a.Invoke(t);
+      var nextV := next;
+      if stop(nextV) {
+        break;
+      }
+      eventuallyStopsProof.InvokeUntilTerminationMetricDecreased@beforeInvoke(next);
+    }
+  }
+
+  // Dependencies stolen from DafnyStandardLibraries
+  
+  function Max(a: int, b: int): int
+  {
+    if a < b
+    then b
+    else a
+  }
+
+  function Min(a: int, b: int): int
+  {
+    if a < b
+    then a
+    else b
+  }
+
   // Common action invariants
 
   function Inputs<T, R>(history: seq<(T, R)>): seq<T> {
@@ -104,54 +170,118 @@ module {:options "--function-syntax:4"} Std.Actions {
     Seq.Map((e: (T, R)) => e.1, history)
   }
 
-  ghost predicate OnlyProduces<T, R>(i: Action<T, R>, history: seq<(T, R)>, c: R) 
-  {
+  trait {:termination false} ConsumesAllProof<T, R> {
+    ghost function Action(): Action<T, R>
+
+    lemma CanConsumeAll(history: seq<(T, R)>, next: T)
+      requires Action().CanProduce(history)
+      ensures Action().CanConsume(history, next)
+  }
+
+  ghost predicate OnlyProduces<T, R>(i: Action<T, R>, history: seq<(T, R)>, c: R) {
     i.CanProduce(history) <==> forall e <- history :: e.1 == c
   }
 
-  ghost predicate CanConsumeAll<T(!new), R(!new)>(a: Action<T, R>, input: seq<T>) 
-  {
-    forall i | 0 < i < |input| ::
-      var consumed := input[..(i - 1)];
-      var next := input[i];
-      forall history | a.CanProduce(history) && Inputs(history) == consumed :: a.CanConsume(history, next)
+  ghost predicate Terminated<T>(s: seq<T>, stop: T -> bool, n: nat) {
+    forall i | 0 <= i < |s| :: n <= i <==> stop(s[i])
   }
 
-  ghost predicate Terminated<T>(s: seq<T>, c: T, n: nat) {
-    forall i | 0 <= i < |s| :: n <= i <==> s[i] == c
-  }
+  lemma TerminatedDistributes<T>(left: seq<T>, right: seq<T>, stop: T -> bool, n: nat)
+    requires Terminated(left, stop, |left|)
+    requires Terminated(right, stop, n)
+    ensures Terminated(left + right, stop, |left| + n)
+  {}
 
-  lemma TerminatedUndistributes<T>(left: seq<T>, right: seq<T>, c: T, n: nat)
-    requires Terminated(left + right, c, n)
-    ensures Terminated(left, c, n)
-    ensures Terminated(right, c, Math.Max(0, n - |left|))
+  lemma TerminatedUndistributes<T>(left: seq<T>, right: seq<T>, stop: T -> bool, n: nat)
+    requires Terminated(left + right, stop, n)
+    ensures Terminated(left, stop, n)
+    ensures Terminated(right, stop, Max(0, n - |left|))
   {
     assert forall i | 0 <= i < |left| :: left[i] == (left + right)[i];
     assert forall i | 0 <= i < |right| :: right[i] == (left + right)[i + |left|];
   }
 
-  // TODO: generalize to "EventuallyProducesSequence"?
-  ghost predicate ProducesTerminatedBy<T(!new), R(!new)>(i: Action<T, R>, c: R, limit: nat) {
-    forall history: seq<(T, R)> | i.CanProduce(history) 
-      :: exists n: nat | n <= limit :: Terminated(Outputs(history), c, n)
+  trait {:termination false} ProducesTerminatedProof<T, R> extends ConsumesAllProof<T, R> {
+
+    ghost function FixedInput(): T
+    ghost function StopFn(): R -> bool
+    ghost function Limit(): nat
+
+    lemma ProducesTerminated(history: seq<(T, R)>) 
+      requires Action().CanProduce(history) 
+      requires (forall i <- Inputs(history) :: i == FixedInput())
+      ensures exists n: nat | n <= Limit() :: Terminated(Outputs(history), StopFn(), n)
+
+    // Termination metric
+    ghost function Remaining(): nat
+      requires Action().Valid()
+      requires forall i <- Action().Consumed() :: i == FixedInput()
+      reads Action().Repr
+    {
+      ProducesTerminated(Action().history);
+      var n: nat :| n <= Limit() && Terminated(Action().Produced(), StopFn(), n);
+      TerminatedDefinesNonTerminalCount(Action().Produced(), StopFn(), n);
+      Limit() - NonTerminalCount(Action().Produced(), StopFn())
+    }
+
+    twostate lemma InvokeUntilTerminationMetricDecreased(new nextProduced: R)
+      requires old(Action().Valid())
+      requires Action().Valid()
+      requires forall i <- old(Action().Consumed()) :: i == FixedInput()
+      requires Action().Consumed() == old(Action().Consumed()) + [FixedInput()]
+      requires Action().Produced() == old(Action().Produced()) + [nextProduced]
+      requires !StopFn()(nextProduced)
+      ensures Remaining() < old(Remaining())
+    {
+      var before := old(Action().Produced());
+      var after := Action().Produced();
+      ProducesTerminated(old(Action().history));
+      var n: nat :| n <= Limit() && Terminated(before, StopFn(), n);
+      ProducesTerminated(Action().history);
+      var m: nat :| m <= Limit() && Terminated(after, StopFn(), m);
+      if n < |before| {
+        assert StopFn()(before[|before| - 1]);
+        assert !StopFn()(Action().Produced()[|Action().Produced()| - 1]);
+        assert |Action().Produced()| <= m;
+        assert !StopFn()(Action().Produced()[|before| - 1]);
+        assert false;
+      } else {
+        TerminatedDefinesNonTerminalCount(before, StopFn(), n);
+        assert NonTerminalCount(before, StopFn()) <= n;
+        TerminatedDistributes(before, [nextProduced], StopFn(), 1);
+        assert Terminated(after, StopFn(), |after|);
+        TerminatedDefinesNonTerminalCount(after, StopFn(), |after|);
+      }
+    }
   }
 
-  // Class of actions whose precondition doesn't depend on history (probably needs a better name)
-  ghost predicate ContextFree<T(!new), R(!new)>(a: Action<T, R>, p: T -> bool) {
-    forall history, next | a.CanProduce(history)
-      :: a.CanConsume(history, next) <==> p(next)
+  function NonTerminalCount<T>(produced: seq<T>, stop: T -> bool): nat {
+    if |produced| == 0 || stop(produced[0]) then
+      0
+    else
+      1 + NonTerminalCount(produced[1..], stop)
   }
 
-  // Aggregators
+  lemma TerminatedDefinesNonTerminalCount<T>(s: seq<T>, stop: T -> bool, n: nat) 
+    requires Terminated(s, stop, n)
+    ensures NonTerminalCount(s, stop) == Min(|s|, n)
+  {
+    if n == 0 || |s| == 0 {
+    } else {
+      if stop(s[0]) {
+      } else {
+        assert 1 <= NonTerminalCount(s, stop);
+        TerminatedDefinesNonTerminalCount(s[1..], stop, n - 1);
+      }
+    }
+  }
+  
+  class FunctionAction<T, R> extends Action<T, R> {
 
-  type IAggregator<T> = Action<T, ()>
-  type Aggregator<T(!new)> = a: Action<T, bool> | exists limit :: ProducesTerminatedBy(a, false, limit) witness *
+    // TODO: Can we support ~>?
+    const f: T --> R
 
-  class ArrayAggregator<T> extends Action<T, ()> {
-
-    var storage: DynamicArray<T>
-
-    ghost predicate Valid() 
+    ghost predicate Valid()
       reads this, Repr 
       ensures Valid() ==> this in Repr 
       ensures Valid() ==> 
@@ -159,68 +289,239 @@ module {:options "--function-syntax:4"} Std.Actions {
       decreases height, 0
     {
       && this in Repr
-      && storage in Repr
-      && this !in storage.Repr
-      && storage.Repr <= Repr
-      && storage.Valid?()
-      && Consumed() == storage.items
+      && CanProduce(history)
+      && Produced() == Seq.Map(f, Consumed())
     }
 
-    constructor() 
+    constructor(f: T -> R) 
       ensures Valid()
-      ensures fresh(Repr - {this})
+      ensures this.f == f
+      ensures fresh(Repr)
       ensures history == []
-    {
-      var a := new DynamicArray();
+    { 
+      this.f := f;
 
       history := [];
-      height := 1;
-      Repr := {this} + {a} + a.Repr;
-      this.storage := a;
+      Repr := {this};
     }
 
-    ghost predicate CanConsume(history: seq<(T, ())>, next: T)
+    ghost predicate CanConsume(history: seq<(T, R)>, next: T)
+      requires CanProduce(history)
       decreases height
     {
-      true
+      f.requires(next)
     }
-    ghost predicate CanProduce(history: seq<(T, ())>)
+    ghost predicate CanProduce(history: seq<(T, R)>)
       decreases height
     {
-      true
+      forall e <- history :: f.requires(e.0) && e.1 == f(e.0)
     }
 
-    method Invoke(t: T) returns (r: ()) 
+    method Invoke(t: T) returns (r: R) 
       requires Requires(t)
       reads Reads(t)
       modifies Modifies(t)
       decreases Decreases(t).Ordinal()
       ensures Ensures(t, r)
     {
-      storage.Push(t);
-
-      r := ();
-      Update(t, r);
-      Repr := {this} + {storage} + storage.Repr;
       assert Valid();
+      r := f(t);
+
+      Update(t, r);
+    }
+
+    method RepeatUntil(t: T, stop: R -> bool, ghost eventuallyStopsProof: ProducesTerminatedProof<T, R>)
+      requires Valid()
+      requires eventuallyStopsProof.Action() == this
+      requires eventuallyStopsProof.FixedInput() == t
+      requires eventuallyStopsProof.StopFn() == stop
+      requires forall i <- Consumed() :: i == t
+      reads Reads(t)
+      modifies Repr
+      decreases Repr
+      ensures Valid()
+    {
+      DefaultRepeatUntil(this, t, stop, eventuallyStopsProof);
     }
   }
 
-  method {:rlimit 0} AggregatorExample() {
-    var a := new ArrayAggregator();
-    var _ := a.Invoke(1);
-    var _ := a.Invoke(2);
-    var _ := a.Invoke(3);
-    var _ := a.Invoke(4);
-    var _ := a.Invoke(5);
-    assert a.storage.items == [1, 2, 3, 4, 5];
+  class FunctionalEnumerator<S, T> extends Action<(), Option<T>> {
+
+    const stepFn: S -> Option<(S, T)>
+    var state: S
+
+    ghost predicate Valid() 
+      reads this, Repr 
+      ensures Valid() ==> this in Repr 
+      ensures Valid() ==> CanProduce(history)
+      decreases height, 0
+    {
+      this in Repr
+    }
+
+    constructor(state: S, stepFn: S -> Option<(S, T)>) {
+      this.state := state;
+      this.stepFn := stepFn;
+    }
+
+    ghost predicate CanConsume(history: seq<((), Option<T>)>, next: ())
+      decreases height
+    {
+      true
+    }
+    ghost predicate CanProduce(history: seq<((), Option<T>)>)
+      decreases height
+    {
+      true
+    }
+
+    method Invoke(t: ()) returns (r: Option<T>) 
+      requires Requires(t)
+      reads Reads(t)
+      modifies Modifies(t)
+      decreases Decreases(t).Ordinal()
+      ensures Ensures(t, r)
+    {
+      var next := stepFn(state);
+      match next {
+        case Some(result) => {
+          var (newState, result') := result;
+          state := newState;
+          r := Some(result');
+        }
+        case None => {
+          r := None;
+        }
+      }
+      Update(t, r);
+    }
+
+    method RepeatUntil(t: (), stop: Option<T> -> bool, ghost eventuallyStopsProof: ProducesTerminatedProof<(), Option<T>>)
+      requires Valid()
+      requires eventuallyStopsProof.Action() == this
+      requires eventuallyStopsProof.FixedInput() == t
+      requires eventuallyStopsProof.StopFn() == stop
+      requires forall i <- Consumed() :: i == t
+      reads Reads(t)
+      modifies Repr
+      decreases Repr
+      ensures Valid()
+    {
+      DefaultRepeatUntil(this, t, stop, eventuallyStopsProof);
+    }
+  }
+  
+  class Box {
+    const i: nat
+
+    constructor(i: nat) 
+      reads {}
+      ensures this.i == i
+    {
+      this.i := i;
+    }
+  }
+
+  function SeqRange(n: nat): seq<nat> {
+    seq(n, i => i)
+  }
+
+  lemma SeqRangeIncr(prefix: seq<nat>, n: nat)
+    requires prefix == SeqRange(n)
+    ensures prefix + [n] == SeqRange(n + 1) 
+  {}
+
+  class BoxEnumerator extends Action<(), Box> {
+
+    var nextValue: nat
+
+    ghost predicate Valid() 
+      reads this, Repr 
+      ensures Valid() ==> this in Repr 
+      ensures Valid() ==> CanProduce(history)
+      decreases height, 0
+    {
+      && this in Repr
+      && CanProduce(history)
+      && nextValue == |history|
+    }
+
+    constructor() 
+      ensures Valid()
+      ensures fresh(Repr)
+      ensures history == []
+    {
+      nextValue := 0;
+      history := [];
+      Repr := {this};
+      height := 1;
+    }
+
+    ghost predicate CanConsume(history: seq<((), Box)>, next: ())
+      decreases height
+    {
+      true
+    }
+    ghost predicate CanProduce(history: seq<((), Box)>)
+      decreases height
+    {
+      Seq.Map((b: Box) => b.i, Outputs(history)) == SeqRange(|history|)
+    }
+
+    method Invoke(t: ()) returns (r: Box) 
+      requires Requires(t)
+      reads Reads(t)
+      modifies Modifies(t)
+      decreases Decreases(t).Ordinal()
+      ensures Ensures(t, r)
+    {
+      ghost var producedBefore := Produced();
+
+      r := new Box(nextValue);
+      Update(t, r);
+      Repr := {this};
+      nextValue := nextValue + 1;
+
+      SeqRangeIncr(Seq.Map((b: Box) => b.i, producedBefore), |producedBefore|);
+      assert Valid();
+    }
+
+    method RepeatUntil(t: (), stop: Box -> bool, ghost eventuallyStopsProof: ProducesTerminatedProof<(), Box>)
+      requires Valid()
+      requires eventuallyStopsProof.Action() == this
+      requires eventuallyStopsProof.FixedInput() == t
+      requires eventuallyStopsProof.StopFn() == stop
+      requires forall i <- Consumed() :: i == t
+      reads Reads(t)
+      modifies Repr
+      decreases Repr
+      ensures Valid()
+    {
+      DefaultRepeatUntil(this, t, stop, eventuallyStopsProof);
+    }
+  }
+
+  method {:rlimit 0} BoxEnumeratorExample() {
+    var enum: BoxEnumerator := new BoxEnumerator();
+    assert |enum.Produced()| == 0;
+    var a := enum.Invoke(());
+
+    assert enum.Produced() == [a];
+    assert Seq.Map((b: Box) => b.i, enum.Produced()) == SeqRange(1) == [0];
+    // assert a.i == 0;
+    
+    // var b := enum.Invoke(());
+    // var c := enum.Invoke(());
+    // var d := enum.Invoke(());
+    // var e := enum.Invoke(());
+
   }
 
   // Other primitives/examples todo:
   //  * Promise-like single-use Action<T, ()> to capture a value for reading later
-  //  * Eliminate all the (!new) restrictions - look into "older" parameters?
-  //    * How to state the invariant that a constructor as an action creates a new object every time?
-  //      * Lemma that takes produced as input, instead of forall produced?
+  //  * datatype/codatatype-based enumerations
+  //  * How to state the invariant that a constructor as an action creates a new object every time?
+  //    * Lemma that takes produced as input, instead of forall produced?
   //  * Enumerable ==> defines e.Enumerator()
   //    * BUT can have infinite containers, probably need IEnumerable as well? (different T for the Action)
   //  * Expressing that an Action "Eventually produces something" (look at how VMC models this for randomness)
@@ -229,5 +530,9 @@ module {:options "--function-syntax:4"} Std.Actions {
   //  * Example of adapting an iterator
   //  * Example of enumerating all possible values of a type (for test generation)
   //    * Needs to handle infinite types too, hence needs the "eventually produces something" concept
-
+  //  * Document: useful pattern to add an Action<Command, Result> facade
+  //        to a set of methods that participate in a protocol.
+  //        Then you have a history that ties the behavior
+  //        of the methods together,
+  //        supporting constraints on the order of calls etc.
 }
